added alive_alloca for LAA, which is similar to the alive_store to LAS. They should be proved in a more generic way.
proving SAS (store after store). The submission does not need it, and
remove all dead stores by DSE at the very end. SAS allows us to remove
redundant stores while searching LAS/LAA w/o passing code again. SAS
should also be useful for proving GVN.

moved all tactics to trans_tactic, and some lemmas to Core.



git-svn-id: https://webdav.seas.upenn.edu/svn/sol/vol@3664 eef5ea85-cc2e-0410-bd84-0fae1f012da8

src/Transforms/alive_alloca.v
@@ -20,76 +20,56 @@ Require Import trans_tactic.
 
 Import Promotability.
 
-Definition alive_store (sid: id) (v:value) (cs2:cmds) (b:block) (pinfo:PhiInfo)
-  : Prop :=
+Definition alive_alloca (cs2:cmds) (b:block) (pinfo:PhiInfo) : Prop :=
 blockInFdefB b (PI_f pinfo) = true /\
 store_in_cmds (PI_id pinfo) cs2 = false /\
 let '(block_intro _ _ cs _) := b in
 exists cs1, exists cs3,
   cs = 
   cs1 ++ 
-  insn_store sid (PI_typ pinfo) v (value_id (PI_id pinfo)) (PI_align pinfo) :: 
+  insn_alloca (PI_id pinfo) (PI_typ pinfo) (PI_num pinfo) (PI_align pinfo) :: 
   cs2 ++ 
   cs3.
 
-Record StoreInfo (pinfo: PhiInfo) := mkStoreInfo {
-  SI_id : id;
-  SI_value : value;
-  SI_tail : cmds;
-  SI_block : block;
-  SI_alive : alive_store SI_id SI_value SI_tail SI_block pinfo
+Record AllocaInfo (pinfo: PhiInfo) := mkAllocaInfo {
+  AI_tail : cmds;
+  AI_block : block;
+  AI_alive : alive_alloca AI_tail AI_block pinfo
 }.
 
-Lemma storeinfo_doesnt_use_promotable_allocas: forall pinfo stinfo 
-  (Huniq: uniqFdef (PI_f pinfo)),
-  WF_PhiInfo pinfo -> SI_value pinfo stinfo <> value_id (PI_id pinfo).
-Proof.
-  intros.
-  destruct stinfo. simpl in *.
-  destruct SI_block0.
-  destruct SI_alive0 as [J1 [J2 [cs1 [cs2 J3]]]]; subst.
-  eapply IngetCmdsIDs__lookupCmdViaIDFromFdef in J1; eauto using in_middle.
-    apply WF_PhiInfo_spec3 in J1; auto.
-    intro EQ; subst.    
-    assert (G:=@valueEqB_refl (value_id (PI_id pinfo))).
-    destruct (valueEqB (value_id (PI_id pinfo)) (value_id (PI_id pinfo)));
-      simpl in *; try congruence.
-Qed.
-
-Definition wf_defs (pinfo:PhiInfo) (stinfo: StoreInfo pinfo) TD M gl (lc:DGVMap)
+Definition wf_defs (pinfo:PhiInfo) (alinfo: AllocaInfo pinfo) TD M gl (lc:DGVMap)
   : Prop :=
 forall gvsa gvsv
   (Hlkpa: lookupAL _ lc (PI_id pinfo) = Some gvsa)
-  (Hlkpv: Opsem.getOperandValue TD (SI_value pinfo stinfo) lc gl 
-    = Some gvsv),
+  (Hlkpv: Opsem.getOperandValue TD (value_const (const_undef (PI_typ pinfo))) lc
+     gl = Some gvsv),
   mload TD M gvsa (PI_typ pinfo) (PI_align pinfo) = Some gvsv.
 
-Definition follow_alive_store (pinfo:PhiInfo) (stinfo: StoreInfo pinfo)
+Definition follow_alive_alloca (pinfo:PhiInfo) (alinfo: AllocaInfo pinfo)
   (cs:cmds) : Prop :=
-let '(block_intro _ _ cs0 _) := SI_block pinfo stinfo in
+let '(block_intro _ _ cs0 _) := AI_block pinfo alinfo in
 forall cs1 cs3, 
   cs0 = 
     cs1 ++ 
-    insn_store (SI_id pinfo stinfo) (PI_typ pinfo) (SI_value pinfo stinfo) 
-      (value_id (PI_id pinfo)) (PI_align pinfo) ::
-    SI_tail pinfo stinfo ++ 
+    insn_alloca (PI_id pinfo) (PI_typ pinfo) (PI_num pinfo) (PI_align pinfo) ::
+    AI_tail pinfo alinfo ++ 
     cs3 ->
   (exists csa, exists csb, 
-    cs = csb ++ cs3 /\ SI_tail pinfo stinfo = csa ++ csb).
+    cs = csb ++ cs3 /\ AI_tail pinfo alinfo = csa ++ csb).
 
-Lemma follow_alive_store_cons: forall pinfo stinfo c cs l0 ps0 cs0 tmn0 
-  (Huniq:uniqFdef (PI_f pinfo)),
-  block_intro l0 ps0 (cs0++c::cs) tmn0 = SI_block pinfo stinfo ->
+Lemma follow_alive_alloca_cons: forall pinfo alinfo c cs l0 ps0 cs0 tmn0 
+  (Huniq:uniqFdef (PI_f pinfo)) (Hneq: getCmdLoc c <> PI_id pinfo),
+  block_intro l0 ps0 (cs0++c::cs) tmn0 = AI_block pinfo alinfo ->
   store_in_cmd (PI_id pinfo) c = false ->
-  follow_alive_store pinfo stinfo cs ->
-  follow_alive_store pinfo stinfo (c::cs).
+  follow_alive_alloca pinfo alinfo cs ->
+  follow_alive_alloca pinfo alinfo (c::cs).
 Proof.
-  unfold follow_alive_store.
+  unfold follow_alive_alloca.
   intros.
-  destruct stinfo. simpl in *.
-  unfold alive_store in SI_alive0.
-  destruct SI_block0.
-  destruct SI_alive0 as [J1 [J2 [cs1 [cs3 J3]]]]; subst.
+  destruct alinfo. simpl in *.
+  unfold alive_alloca in AI_alive0.
+  destruct AI_block0.
+  destruct AI_alive0 as [J1 [J2 [cs1 [cs3 J3]]]]; subst.
   intros.
   assert (cs1 = cs2 /\ cs3 = cs4) as J. 
     apply uniqFdef__blockInFdefB__nodup_cmds in J1; auto.
@@ -103,8 +83,8 @@ Proof.
   subst. inv H.
   rewrite_env 
     (((cs2 ++
-       insn_store SI_id0 (PI_typ pinfo) SI_value0 (value_id (PI_id pinfo))
-         (PI_align pinfo) :: csa) ++ csb) ++ cs4) in H4.
+       insn_alloca (PI_id pinfo) (PI_typ pinfo) 
+               (PI_num pinfo) (PI_align pinfo) :: csa) ++ csb) ++ cs4) in H4.
   rewrite_env (((cs0 ++ [c]) ++ csb) ++ cs4) in H4.
   apply app_inv_tail in H4.
   apply app_inv_tail in H4.
@@ -112,8 +92,7 @@ Proof.
     simpl_env in H4.
     apply app_inj_tail in H4.
     destruct H4 as [EQ1 EQ2]; subst.
-    simpl in H0. 
-    destruct (id_dec (PI_id pinfo) (PI_id pinfo)); simpl in H0; congruence.
+    contradict Hneq; auto.
 
     assert (exists csa', exists c2, [c0] ++ csa = csa' ++ [c2]) as EQ. 
       apply head_tail_commut.
@@ -121,8 +100,8 @@ Proof.
     simpl_env in H4.
     rewrite EQ in H4.
     rewrite_env ((cs2 ++
-      insn_store SI_id0 (PI_typ pinfo) SI_value0 (value_id (PI_id pinfo))
-        (PI_align pinfo) :: csa') ++ [c2]) in H4.
+      insn_alloca (PI_id pinfo) (PI_typ pinfo) 
+               (PI_num pinfo) (PI_align pinfo) :: csa') ++ [c2]) in H4.
     apply app_inj_tail in H4.
     destruct H4 as [EQ1 EQ2]; subst.
     exists csa'. exists (c2::csb). simpl_env. 
@@ -131,34 +110,35 @@ Proof.
     split; auto.
 Qed.
 
-Definition wf_ExecutionContext (pinfo:PhiInfo) (stinfo: StoreInfo pinfo) TD M gl
+Definition wf_ExecutionContext (pinfo:PhiInfo) (alinfo: AllocaInfo pinfo) TD M gl
   (ec:Opsem.ExecutionContext) : Prop :=
 Opsem.CurFunction ec = PI_f pinfo ->
-Opsem.CurBB ec = SI_block pinfo stinfo ->
-follow_alive_store pinfo stinfo (Opsem.CurCmds ec) ->
-wf_defs pinfo stinfo TD M gl (Opsem.Locals ec).
+Opsem.CurBB ec = AI_block pinfo alinfo ->
+follow_alive_alloca pinfo alinfo (Opsem.CurCmds ec) ->
+wf_defs pinfo alinfo TD M gl (Opsem.Locals ec).
 
-Fixpoint wf_ECStack (pinfo:PhiInfo) (stinfo: StoreInfo pinfo) TD M gl 
+Fixpoint wf_ECStack (pinfo:PhiInfo) (alinfo: AllocaInfo pinfo) TD M gl 
   (ecs:Opsem.ECStack) : Prop :=
 match ecs with
 | nil => True
 | ec::ecs' => 
-    wf_ExecutionContext pinfo stinfo TD M gl ec /\
-    wf_ECStack pinfo stinfo TD M gl ecs'
+    wf_ExecutionContext pinfo alinfo TD M gl ec /\
+    wf_ECStack pinfo alinfo TD M gl ecs'
 end.
 
-Definition wf_State (pinfo:PhiInfo) (stinfo: StoreInfo pinfo) 
+Definition wf_State (pinfo:PhiInfo) (alinfo: AllocaInfo pinfo) 
   (cfg:OpsemAux.Config) (S:Opsem.State) : Prop :=
-wf_ECStack pinfo stinfo (OpsemAux.CurTargetData cfg) (Opsem.Mem S) 
+wf_ECStack pinfo alinfo (OpsemAux.CurTargetData cfg) (Opsem.Mem S) 
   (OpsemAux.Globals cfg) (Opsem.ECS S).
 
+(* its proof is same to alive_store.v *)
 Lemma free_allocas_preserves_wf_defs: forall pinfo TD Mem lc' als0 als Mem'
-  gl stinfo maxb, 
+  gl alinfo maxb, 
   Promotability.wf_defs maxb pinfo TD Mem lc' als0 ->
-  wf_defs pinfo stinfo TD Mem gl lc' ->
+  wf_defs pinfo alinfo TD Mem gl lc' ->
   NoDup (als ++ als0) ->
   free_allocas TD Mem als = ret Mem' ->
-  wf_defs pinfo stinfo TD Mem' gl lc'.
+  wf_defs pinfo alinfo TD Mem' gl lc'.
 Proof.
   intros. unfold wf_defs in *. intros.
   assert (Hlkpa':=Hlkpa).
@@ -170,24 +150,17 @@ Proof.
   eapply free_allocas_preserves_mload; eauto.
 Qed.
 
-Lemma wf_defs_updateAddAL: forall pinfo stinfo TD M lc' i1 gv1 gl
-  (Hwfpi: WF_PhiInfo pinfo) (Huniq: uniqFdef (PI_f pinfo))
-  (HwfDef: wf_defs pinfo stinfo TD M gl lc') 
-  (Hneq: i1 <> PI_id pinfo) 
-  (Hnouse: used_in_value i1 (SI_value pinfo stinfo) = false),
-  wf_defs pinfo stinfo TD M gl (updateAddAL _ lc' i1 gv1).
+Lemma wf_defs_updateAddAL: forall pinfo alinfo TD M lc' i1 gv1 gl
+  (HwfDef: wf_defs pinfo alinfo TD M gl lc') 
+  (Hneq: i1 <> PI_id pinfo),
+  wf_defs pinfo alinfo TD M gl (updateAddAL _ lc' i1 gv1).
 Proof.
   intros. unfold wf_defs in *. intros.
   rewrite <- lookupAL_updateAddAL_neq in Hlkpa; auto.
-  eapply HwfDef; eauto.
-  apply storeinfo_doesnt_use_promotable_allocas with (stinfo:=stinfo) in Hwfpi; 
-    auto.
-  destruct (SI_value pinfo stinfo); simpl in *; auto.
-  destruct (id_dec i0 i1); simpl in Hnouse; try congruence.
-  rewrite <- lookupAL_updateAddAL_neq in Hlkpv; auto.
 Qed.
 
-Lemma free_allocas_preserves_wf_ECStack: forall maxb pinfo stinfo td als gl ECs 
+(* its proof is same to alive_store.v *)
+Lemma free_allocas_preserves_wf_ECStack: forall maxb pinfo alinfo td als gl ECs 
   Mem Mem'
   (HwfECs : Promotability.wf_ECStack maxb pinfo td Mem ECs)
   (Hwfpi: WF_PhiInfo pinfo)
@@ -195,9 +168,9 @@ Lemma free_allocas_preserves_wf_ECStack: forall maxb pinfo stinfo td als gl ECs
                   (fun ec : Opsem.ExecutionContext =>
                    let '{| Opsem.Allocas := als |} := ec in als)
                    ECs)))
-  (Hwf: wf_ECStack pinfo stinfo td Mem gl ECs)
+  (Hwf: wf_ECStack pinfo alinfo td Mem gl ECs)
   (Hfrees: free_allocas td Mem als = ret Mem'),
-  wf_ECStack pinfo stinfo td Mem' gl ECs.
+  wf_ECStack pinfo alinfo td Mem' gl ECs.
 Proof.
   induction ECs as [|[]]; simpl; intros; auto.
     destruct Hwf as [J1 J2].
@@ -216,40 +189,37 @@ Proof.
       eapply free_allocas_preserves_wf_defs in G3; eauto. 
 Qed.
 
-Lemma follow_alive_store_at_beginning_false: forall (pinfo : PhiInfo) 
-  (stinfo : StoreInfo pinfo) (l' : l) (ps' : phinodes) (cs' : cmds) 
+Lemma follow_alive_alloca_at_beginning_false: forall (pinfo : PhiInfo) 
+  (alinfo : AllocaInfo pinfo) (l' : l) (ps' : phinodes) (cs' : cmds) 
   (tmn' : terminator) 
-  (J2 : block_intro l' ps' cs' tmn' = SI_block pinfo stinfo)
-  (J3 : follow_alive_store pinfo stinfo cs'),
+  (J2 : block_intro l' ps' cs' tmn' = AI_block pinfo alinfo)
+  (J3 : follow_alive_alloca pinfo alinfo cs'),
   False.
 Proof.
   intros.
-  unfold follow_alive_store in J3.
+  unfold follow_alive_alloca in J3.
   rewrite <- J2 in J3.
-  destruct stinfo. simpl in *.
-  rewrite <- J2 in SI_alive0.
-  destruct SI_alive0 as [_ [_ [cs1 [cs3 J]]]].
+  destruct alinfo. simpl in *.
+  rewrite <- J2 in AI_alive0.
+  destruct AI_alive0 as [_ [_ [cs1 [cs3 J]]]].
   assert (J':=J).
   apply J3 in J.
   destruct J as [csa [csb [EQ1 EQ2]]]; subst.
   rewrite_env (
     (cs1 ++
-     insn_store SI_id0 (PI_typ pinfo) 
-       SI_value0 (value_id (PI_id pinfo)) 
-       (PI_align pinfo) :: (csa ++ csb)) ++ cs3
+     insn_alloca (PI_id pinfo) (PI_typ pinfo) (PI_num pinfo)
+         (PI_align pinfo) :: (csa ++ csb)) ++ cs3
     ) in J'.
   apply app_inv_tail in J'. 
   rewrite_env (
     (cs1 ++
-     insn_store SI_id0 (PI_typ pinfo) 
-       SI_value0 (value_id (PI_id pinfo)) 
-       (PI_align pinfo) :: csa) ++ csb
+     insn_alloca (PI_id pinfo) (PI_typ pinfo) (PI_num pinfo)
+         (PI_align pinfo) :: csa) ++ csb
     ) in J'.
   symmetry in J'.
   apply app_inv_tail_nil in J'.
   assert (
-    In (insn_store SI_id0 (PI_typ pinfo) 
-         SI_value0 (value_id (PI_id pinfo)) 
+    In (insn_alloca (PI_id pinfo) (PI_typ pinfo) (PI_num pinfo)
          (PI_align pinfo)) nil) as Hin.
     rewrite <- J'. apply in_middle.
   inv Hin.
@@ -264,66 +234,11 @@ match goal with
   split; try solve [
     auto |
     intros J1 J2 J3; simpl in *; subst;
-    eapply follow_alive_store_at_beginning_false in J3; eauto;
+    eapply follow_alive_alloca_at_beginning_false in J3; eauto;
     inv J3]
 end.
 
-Lemma alive_store_doesnt_use_its_followers: forall l1 ps1 cs1' c cs tmn id0
-  pinfo stinfo ifs s m (Huniq: uniqFdef (PI_f pinfo)),
-  wf_fdef ifs s m (PI_f pinfo) -> 
-  block_intro l1 ps1 (cs1' ++ c :: cs) tmn = SI_block pinfo stinfo ->
-  getCmdID c = Some id0 ->
-  follow_alive_store pinfo stinfo (c::cs) ->
-  used_in_value id0 (SI_value pinfo stinfo) = false.
-Proof.
-  intros.
-  unfold follow_alive_store in H2.
-  rewrite <- H0 in H2.
-  destruct stinfo. simpl in *. 
-  rewrite <- H0 in SI_alive0.
-  destruct SI_alive0 as [J1 [J5 [cs1 [cs2 J4]]]].
-  assert (J4':=J4).
-  apply H2 in J4. clear H2.
-  destruct J4 as [csa [csb [EQ1 EQ2]]]; subst.
-  rewrite EQ1 in J4'.
-  rewrite_env ((cs1' ++ csb) ++ cs2) in J4'.
-  rewrite_env (((cs1 ++ insn_store SI_id0 (PI_typ pinfo) SI_value0 
-                          (value_id (PI_id pinfo)) (PI_align pinfo) :: 
-                csa) ++ csb) ++ cs2) in J4'.
-  apply app_inv_tail in J4'.
-  apply app_inv_tail in J4'. subst.
-  simpl_env in J1. simpl in J1.
-  assert (J1':=J1).
-  eapply wf_fdef__wf_cmd in J1; eauto using in_middle.
-  inv J1.
-  inv H14. 
-  destruct SI_value0; auto.
-  apply wf_operand_list__elim with (id1:=i0)(f1:=PI_f pinfo)
-    (b1:=block_intro l1 ps1
-                  (cs1 ++
-                   insn_store SI_id0 (PI_typ pinfo) 
-                     (value_id i0) (value_id (PI_id pinfo)) 
-                     (PI_align pinfo) :: csa ++ c :: cs) tmn)
-    (insn1:=insn_cmd
-                  (insn_store SI_id0 (PI_typ pinfo) 
-                     (value_id i0) (value_id (PI_id pinfo)) 
-                     (PI_align pinfo))) in H8; auto.
-    inv H8.
-    apply inGetBlockIDs__lookupBlockViaIDFromFdef with (id1:=i0) in J1'; auto.
-      rewrite J1' in H14. inv H14.
-      destruct H16 as [H16 | [H16 | H16]].
-        admit. (* >> *)
-
-        admit. (* ~ l >> l *)
-
-        admit. (* reach *)
-
-      simpl. admit. (* Hin *)
-      
-    admit. (* Hin *)
-Qed.
-
-Lemma preservation_return : forall maxb pinfo stinfo (HwfPI : WF_PhiInfo pinfo)  
+Lemma preservation_return : forall maxb pinfo alinfo (HwfPI : WF_PhiInfo pinfo)  
   F B rid RetTy Result lc F' B' c' cs' tmn' lc' EC Mem als als' cfg
   EC1 EC2 
   (EQ1:EC1 = {| Opsem.CurFunction := F;
@@ -349,10 +264,10 @@ Lemma preservation_return : forall maxb pinfo stinfo (HwfPI : WF_PhiInfo pinfo)
   (H1 : Opsem.returnUpdateLocals 
           (OpsemAux.CurTargetData cfg) c' 
             Result lc lc' (OpsemAux.Globals cfg) = ret lc'')
-  (HwfS1 : wf_State pinfo stinfo cfg
+  (HwfS1 : wf_State pinfo alinfo cfg
             {| Opsem.ECS := EC1 :: EC2 :: EC;
                Opsem.Mem := Mem |}),
-  wf_State pinfo stinfo cfg
+  wf_State pinfo alinfo cfg
      {| Opsem.ECS :=
              {| Opsem.CurFunction := F';
                 Opsem.CurBB := B';
@@ -394,7 +309,9 @@ Proof.
     unfold wf_ExecutionContext in *. simpl in Hinscope1, Hinscope2.
     assert (J2':=J2).
     assert (uniqFdef (PI_f pinfo)) as Huniq. eauto using wf_system__uniqFdef.
-    apply follow_alive_store_cons in J2; auto.
+    assert (getCmdLoc (insn_call i0 n c t v p) <> PI_id pinfo) as Hneq.
+      admit. (* uniq *)
+    apply follow_alive_alloca_cons in J2; auto.
     assert (J2'':=J2).
     apply Hinscope2 in J2; auto.
     assert (NoDup (als ++ als')) as Hnodup.
@@ -418,9 +335,6 @@ Proof.
         remember (lift_op1 DGVs (fit_gv (los, nts) t) g t) as R2.
         destruct R2; inv H1.
         apply wf_defs_updateAddAL; auto.
-          eapply WF_PhiInfo_spec10 in HBinF1; eauto.
-          eapply alive_store_doesnt_use_its_followers; 
-            eauto using wf_system__wf_fdef.
 
       SSSSSCase "c' defines nothing".
         destruct n; inv HeqR. inv H1. auto.
@@ -431,7 +345,7 @@ Proof.
       apply NoDup_strenthening in Hdisjals; auto.
 Qed.
 
-Lemma preservation_return_void : forall maxb pinfo stinfo 
+Lemma preservation_return_void : forall maxb pinfo alinfo 
   (HwfPI : WF_PhiInfo pinfo)  
   F B rid lc F' B' c' cs' tmn' lc' EC Mem als als' cfg EC1 EC2 
   (EQ1:EC1 = {| Opsem.CurFunction := F;
@@ -454,10 +368,10 @@ Lemma preservation_return_void : forall maxb pinfo stinfo
               Opsem.Mem := Mem |})
   Mem' (H : Instruction.isCallInst c' = true)
   (H0 : free_allocas (OpsemAux.CurTargetData cfg) Mem als = ret Mem')
-  (HwfS1 : wf_State pinfo stinfo cfg
+  (HwfS1 : wf_State pinfo alinfo cfg
             {| Opsem.ECS := EC1 :: EC2 :: EC;
                Opsem.Mem := Mem |}),
-  wf_State pinfo stinfo cfg
+  wf_State pinfo alinfo cfg
      {| Opsem.ECS :=
              {| Opsem.CurFunction := F';
                 Opsem.CurBB := B';
@@ -497,7 +411,9 @@ Proof.
     destruct c'; try solve [inversion H].
     unfold wf_ExecutionContext in *. simpl in Hinscope1, Hinscope2.
     assert (J2':=J2).
-    apply follow_alive_store_cons in J2; eauto using wf_system__uniqFdef.
+    assert (getCmdLoc (insn_call i0 n c t v p) <> PI_id pinfo) as Hneq.
+      admit. (* uniq *)
+    apply follow_alive_alloca_cons in J2; eauto using wf_system__uniqFdef.
     apply Hinscope2 in J2; auto.
     assert (NoDup (als ++ als')) as Hnodup.
       rewrite_env 
@@ -520,7 +436,7 @@ Lemma malloc_preserves_wf_EC_at_head : forall pinfo los nts Ps M
   (Hwfpi:WF_PhiInfo pinfo) ifs s als'
   M' gl als lc t mb id0 align0 F gn tsz l1 ps1 cs1' cs tmn 
   (HwfF: wf_fdef ifs s (module_intro los nts Ps) F) (HuniqF: uniqFdef F)
-  (Hal: malloc (los,nts) M tsz gn align0 = ret (M', mb)) stinfo c
+  (Hal: malloc (los,nts) M tsz gn align0 = ret (M', mb)) alinfo c
   (HBinF: blockInFdefB
              (block_intro l1 ps1 (cs1' ++ c :: cs)
                 tmn) F = true)
@@ -530,7 +446,7 @@ Lemma malloc_preserves_wf_EC_at_head : forall pinfo los nts Ps M
            | insn_malloc _ _ _ _ | insn_alloca _ _ _ _ => True
            | _ => False
            end)
-  (Hinscope : wf_ExecutionContext pinfo stinfo (los,nts) M gl
+  (Hinscope : wf_ExecutionContext pinfo alinfo (los,nts) M gl
                {|
                Opsem.CurFunction := F;
                Opsem.CurBB := block_intro l1 ps1
@@ -540,7 +456,7 @@ Lemma malloc_preserves_wf_EC_at_head : forall pinfo los nts Ps M
                Opsem.Terminator := tmn;
                Opsem.Locals := lc;
                Opsem.Allocas := als |}),
-  wf_ExecutionContext pinfo stinfo (los,nts) M' gl
+  wf_ExecutionContext pinfo alinfo (los,nts) M' gl
     {|
     Opsem.CurFunction := F;
     Opsem.CurBB := block_intro l1 ps1
@@ -554,65 +470,57 @@ Proof.
   intros.
   intros J1 J2 J3. simpl in J1, J2, J3. simpl. subst.
   assert (J2':=J2).
-  apply follow_alive_store_cons in J2; auto.
-  assert (used_in_value id0 (SI_value pinfo stinfo) = false) as Hnuse.
-    eapply alive_store_doesnt_use_its_followers; eauto.
-  apply Hinscope in J2; auto. simpl in J2.
-  destruct (fdef_dec (PI_f pinfo) (PI_f pinfo)); try congruence.
-  apply wf_defs_updateAddAL with (i1:=id0)
-    (gv1:=($ blk2GV (los,nts) mb # typ_pointer t $)) in J2; auto.
-    intros gvsa gvsv Hlkpa Hlkpv.
-    eapply J2 in Hlkpv; eauto.
-    eapply malloc_preserves_mload; eauto.
-      destruct (id_dec id0 (PI_id pinfo)); subst; auto.
-      destruct c; tinv Hsort.
-        apply getCmdLoc_getCmdID in Hid; subst.
-        eapply WF_PhiInfo_spec10 in HBinF; eauto.
+  destruct (id_dec id0 (PI_id pinfo)); subst.
+  Case "id0 = PI_id pinfo".
+        destruct c; tinv Hsort.
+        SCase "c = malloc".
+          apply getCmdLoc_getCmdID in Hid; subst.
+          eapply WF_PhiInfo_spec10 in HBinF; eauto.
+            clear - Hid HBinF.
+            contradict Hid; auto.
+    
+        SCase "c = alloca".
+          inv Hid.
+          clear - J2' J3 HwfF Hal. unfold follow_alive_alloca in J3.
+          rewrite <- J2' in J3.
+          destruct alinfo. simpl in *. subst.
+          destruct AI_alive0 as [J1 [J5 [cs1 [cs2 J4]]]].
+          assert (J4':=J4).
+          apply J3 in J4'. clear J3.
+          destruct J4' as [csa [csb [EQ1 EQ2]]]; subst. 
+                    unfold wf_defs. intros.
+          rewrite lookupAL_updateAddAL_eq in Hlkpa. inv Hlkpa.
+          simpl in Hlkpv.
+          rewrite_env (((cs1' ++ [insn_alloca (PI_id pinfo) t0 v a]) ++ csb) 
+                       ++ cs2) in J4.
+          rewrite_env (((cs1 ++
+                       insn_alloca (PI_id pinfo) (PI_typ pinfo) (PI_num pinfo)
+                         (PI_align pinfo) :: 
+                       csa) ++ csb) ++ cs2) in J4.
+          apply app_inv_tail in J4.
+          apply app_inv_tail in J4.
+          admit. (* 1) this is a memory prop. 
+                    2) need to provide the relations between tsz/gn/align0 with
+                         pinfo *)
 
-        inv Hid.
-        clear - J2' J3 HwfF. unfold follow_alive_store in J3.
-        rewrite <- J2' in J3.
-        destruct stinfo. simpl in *. 
-        rewrite <- J2' in SI_alive0.
-        destruct SI_alive0 as [J1 [J5 [cs1 [cs2 J4]]]].
-        assert (J4':=J4).
-        apply J3 in J4. clear J3.
-        destruct J4 as [csa [csb [EQ1 EQ2]]]; subst.
-        rewrite_env (((cs1' ++ [insn_alloca (PI_id pinfo) t0 v a]) ++ csb) 
-                     ++ cs2) in J4'.
-        rewrite_env (((cs1 ++
-                     insn_store SI_id0 (PI_typ pinfo) SI_value0 
-                       (value_id (PI_id pinfo)) (PI_align pinfo) :: 
-                     csa) ++ csb) ++ cs2) in J4'.
-        apply app_inv_tail in J4'.
-        apply app_inv_tail in J4'.
-        destruct csa.
-          simpl_env.
-          apply app_inj_tail in J4'.
-          destruct J4' as [_ A]; inv A.
-
-          assert (exists csa', exists c', [c] ++ csa = csa' ++ [c']) as EQ. 
-            apply head_tail_commut.
-          destruct EQ as [csa' [c' EQ]].
-          rewrite_env (cs1 ++
-                         insn_store SI_id0 (PI_typ pinfo) SI_value0 
-                           (value_id (PI_id pinfo)) (PI_align pinfo) :: 
-                         [c] ++ csa) in J4'.
-          rewrite EQ in J4'.
-          rewrite_env ((cs1 ++
-                         insn_store SI_id0 (PI_typ pinfo) SI_value0 
-                           (value_id (PI_id pinfo)) (PI_align pinfo) :: 
-                         csa') ++ [c'])  in J4'.
-          apply app_inj_tail in J4'.
-          destruct J4' as [A B]; subst.
-          admit. (* >>, see alive_store_doesnt_use_its_followers *)
+  Case "id0 <> PI_id pinfo".
+    apply getCmdLoc_getCmdID in Hid. subst.
+    apply follow_alive_alloca_cons in J2; auto.
+    apply Hinscope in J2; auto. simpl in J2.
+    destruct (fdef_dec (PI_f pinfo) (PI_f pinfo)); try congruence.
+    apply wf_defs_updateAddAL with (i1:=getCmdLoc c)
+      (gv1:=($ blk2GV (los,nts) mb # typ_pointer t $)) in J2; auto.
+      intros gvsa gvsv Hlkpa Hlkpv.
+      eapply J2 in Hlkpv; eauto.
+      eapply malloc_preserves_mload; eauto.
 Qed.
 
+(* its proof is same to alive_store.v *)
 Lemma malloc_preserves_wf_EC_in_tail : forall pinfo td M 
   EC M' gl mb align0 gn tsz 
-  (Hal: malloc td M tsz gn align0 = ret (M', mb)) stinfo
-  (Hinscope : wf_ExecutionContext pinfo stinfo td M gl EC),
-  wf_ExecutionContext pinfo stinfo td M' gl EC.
+  (Hal: malloc td M tsz gn align0 = ret (M', mb)) alinfo
+  (Hinscope : wf_ExecutionContext pinfo alinfo td M gl EC),
+  wf_ExecutionContext pinfo alinfo td M' gl EC.
 Proof.
   intros.
   intros J1 J2 J3. 
@@ -622,11 +530,12 @@ Proof.
   eapply malloc_preserves_mload; eauto.
 Qed.
 
-Lemma malloc_preserves_wf_ECStack_in_tail : forall pinfo stinfo TD M tsz gn 
+(* its proof is same to alive_store.v *)
+Lemma malloc_preserves_wf_ECStack_in_tail : forall pinfo alinfo TD M tsz gn 
   align0 (Hwfpi: WF_PhiInfo pinfo) M' mb gl
   (Hmlc: malloc TD M tsz gn align0 = ret (M', mb)) ECs
-  (Hwf: wf_ECStack pinfo stinfo TD M gl ECs),
-  wf_ECStack pinfo stinfo TD M' gl ECs.
+  (Hwf: wf_ECStack pinfo alinfo TD M gl ECs),
+  wf_ECStack pinfo alinfo TD M' gl ECs.
 Proof.
   induction ECs; simpl; intros; auto.
     destruct Hwf as [J1 J2].
@@ -634,6 +543,7 @@ Proof.
       eapply malloc_preserves_wf_EC_in_tail; eauto.
 Qed.
 
+(* same to alive_store.v *)
 Ltac destruct_ctx_other :=
 match goal with
 | Hwfpp : OpsemPP.wf_State _ _,
@@ -656,14 +566,15 @@ match goal with
   fold Promotability.wf_ECStack in HwfECs'
 end.
 
+(* its proof is same to alive_store.v *)
 Lemma free_preserves_wf_EC_in_tail : forall pinfo td M  EC M' mptr0 
   maxb gl (Hwfg: wf_globals maxb gl)
-  (Hfree: free td M mptr0 = ret M') stinfo mptrs v lc
+  (Hfree: free td M mptr0 = ret M') alinfo mptrs v lc
   (H : Opsem.getOperandValue td v lc gl = ret mptrs)
   (H0 : mptr0 @ mptrs)
-  (Hinscope : wf_ExecutionContext pinfo stinfo td M gl EC)
+  (Hinscope : wf_ExecutionContext pinfo alinfo td M gl EC)
   (Hht : wf_ECStack_head_in_tail maxb pinfo td M lc EC),
-  wf_ExecutionContext pinfo stinfo td M' gl EC.
+  wf_ExecutionContext pinfo alinfo td M' gl EC.
 Proof.
   intros.
   intros J1 J2 J3. 
@@ -674,14 +585,15 @@ Proof.
     eapply operand__no_alias_with__tail; eauto.
 Qed.
 
-Lemma free_preserves_wf_ECStack_in_tail : forall maxb pinfo stinfo TD M  
+(* its proof is same to alive_store.v *)
+Lemma free_preserves_wf_ECStack_in_tail : forall maxb pinfo alinfo TD M  
   (Hwfpi: WF_PhiInfo pinfo) M' gl mptr0 (Hwfg: wf_globals maxb gl)
   (Hfree: free TD M mptr0 = ret M') lc mptrs v
   (H : Opsem.getOperandValue TD v lc gl = ret mptrs)
   (H0 : mptr0 @ mptrs) ECs 
   (Hhts: wf_ECStack_head_tail maxb pinfo TD M lc ECs)
-  (Hwf: wf_ECStack pinfo stinfo TD M gl ECs),
-  wf_ECStack pinfo stinfo TD M' gl ECs.
+  (Hwf: wf_ECStack pinfo alinfo TD M gl ECs),
+  wf_ECStack pinfo alinfo TD M' gl ECs.
 Proof.
   induction ECs; simpl; intros; auto.
     destruct Hwf as [J1 J2].
@@ -693,8 +605,8 @@ Qed.
 
 Lemma preservation_pure_cmd_updated_case : forall (F : fdef)(B : block)
   (lc : DGVMap)(gv3 : GVsT DGVs) (cs : list cmd) (tmn : terminator) id0 c0 Mem0 
-  als ECs pinfo stinfo
-  (HwfPI : WF_PhiInfo pinfo) (Hid : Some id0 = getCmdID c0) cfg maxb EC
+  als ECs pinfo alinfo
+  (HwfPI : WF_PhiInfo pinfo) (Hid : getCmdID c0 = Some id0) cfg maxb EC
   (Heq: EC = {| Opsem.CurFunction := F;
                 Opsem.CurBB := B;
                 Opsem.CurCmds := c0 :: cs;
@@ -707,16 +619,14 @@ Lemma preservation_pure_cmd_updated_case : forall (F : fdef)(B : block)
   (Hnoalias : Promotability.wf_State maxb pinfo cfg
            {| Opsem.ECS := EC :: ECs;
               Opsem.Mem := Mem0 |})
-  (HwfS1 : wf_State pinfo stinfo cfg
+  (HwfS1 : wf_State pinfo alinfo cfg
             {| Opsem.ECS := EC :: ECs;
                Opsem.Mem := Mem0 |})
   (Hnst : store_in_cmd (PI_id pinfo) c0 = false)
   (Hneq :  F = PI_f pinfo -> 
-           B = SI_block pinfo stinfo ->
-           follow_alive_store pinfo stinfo (c0 :: cs) ->
-           (id0 <> PI_id pinfo /\
-           used_in_value id0 (SI_value pinfo stinfo) = false)),
-  wf_State pinfo stinfo cfg
+           B = AI_block pinfo alinfo ->
+           id0 <> PI_id pinfo),
+  wf_State pinfo alinfo cfg
      {|
      Opsem.ECS := {|
             Opsem.CurFunction := F;
@@ -752,29 +662,15 @@ Proof.
     unfold wf_ExecutionContext in *. simpl in Hinscope.
     assert (uniqFdef (PI_f pinfo)) as Huniq. eauto using wf_system__uniqFdef.
     assert (J2':=J2).
-    apply follow_alive_store_cons in J2; auto.
+    apply getCmdLoc_getCmdID in Hid; subst.
+    apply follow_alive_alloca_cons in J2; eauto.
     assert (J2'':=J2).
     apply Hinscope in J2; auto.
-    destruct Hneq as [G1 G2]; auto.
     eapply wf_defs_updateAddAL; eauto.
 Qed.
 
-Lemma mstore_mload_same: forall td Mem mp2 typ1 gv1 align1 Mem',
-  mstore td Mem mp2 typ1 gv1 align1 = ret Mem' ->
-  mload td Mem' mp2 typ1 align1 = ret gv1.
-Proof.
-  intros.
-  apply genericvalues.LLVMgv.store_inv in H.
-  destruct H as [b0 [ofs0 [J1 J4]]].
-  unfold mload.
-  rewrite J1.
-
-  (* We know well-formed typ1 must be flattened. But we should prove that 
-     gv1 must match the list of flattened chunks. !!! *)
-Admitted.
-
 Lemma mstore_preserves_wf_EC_at_head: forall (maxb : Z) (pinfo : PhiInfo) 
-  (stinfo : StoreInfo pinfo) (S : system) td
+  (alinfo : AllocaInfo pinfo) (S : system) td
   (Ps : list product) (gl : GVMap) (fs : GVMap) (Hwfg : wf_globals maxb gl)
   (F : fdef) (lc : Opsem.GVsMap) (sid : id) (t : typ) (align0 : align)
   (v1 : value) (v2 : value) (cs : list cmd) (tmn : terminator) (Mem : mem)
@@ -788,7 +684,7 @@ Lemma mstore_preserves_wf_EC_at_head: forall (maxb : Z) (pinfo : PhiInfo)
   (Hinscope' : if fdef_dec (PI_f pinfo) F
                then Promotability.wf_defs maxb pinfo td Mem lc als
                else True)
-  (Hinscope : wf_ExecutionContext pinfo stinfo td Mem gl
+  (Hinscope : wf_ExecutionContext pinfo alinfo td Mem gl
                {|
                Opsem.CurFunction := F;
                Opsem.CurBB := block_intro l1 ps1
@@ -798,7 +694,7 @@ Lemma mstore_preserves_wf_EC_at_head: forall (maxb : Z) (pinfo : PhiInfo)
                Opsem.Terminator := tmn;
                Opsem.Locals := lc;
                Opsem.Allocas := als |}),
-  wf_ExecutionContext pinfo stinfo td Mem' gl
+  wf_ExecutionContext pinfo alinfo td Mem' gl
      {|
      Opsem.CurFunction := F;
      Opsem.CurBB := block_intro l1 ps1
@@ -814,20 +710,19 @@ Proof.
   remember (store_in_cmd (PI_id pinfo) (insn_store sid t v1 v2 align0)) as R.
   destruct R.
     clear - J2 J3 HeqR H3 H2 H0 H1 H.
-    unfold follow_alive_store in J3.
+    unfold follow_alive_alloca in J3.
     rewrite <- J2 in J3.
-    destruct stinfo. simpl in *.
-    assert (SI_alive0':=SI_alive0).   
-    rewrite <- J2 in SI_alive0'.
-    destruct SI_alive0' as [G1 [G2 [cs1 [cs2 EQ]]]].
+    destruct alinfo. simpl in *.
+    assert (AI_alive0':=AI_alive0).   
+    rewrite <- J2 in AI_alive0'.
+    destruct AI_alive0' as [G1 [G2 [cs1 [cs2 EQ]]]].
     assert (EQ':=EQ).
     apply J3 in EQ. clear J3.
     destruct EQ as [csa [csb [EQ1 EQ2]]]; subst.
     rewrite_env (((cs1' ++ [insn_store sid t v1 v2 align0]) ++ csb) ++ cs2) in 
       EQ'.
-    rewrite_env (((cs1 ++  [insn_store SI_id0 (PI_typ pinfo) SI_value0 
-                 (value_id (PI_id pinfo)) (PI_align pinfo)] ++ csa) ++ csb) ++ 
-                 cs2) in EQ'.
+    rewrite_env (((cs1 ++ [insn_alloca (PI_id pinfo) (PI_typ pinfo) 
+                 (PI_num pinfo) (PI_align pinfo)] ++ csa) ++ csb) ++ cs2) in EQ'.
     apply app_inv_tail in EQ'.
     apply app_inv_tail in EQ'.
     destruct csa.
@@ -835,20 +730,14 @@ Proof.
       apply app_inj_tail in EQ'.
       destruct EQ' as [EQ1 EQ2]; subst.
       inv EQ2. 
-      intros gvsa gvsv Hlkpa Hlkpv. 
-      simpl in *.
-      rewrite H0 in Hlkpa. inv Hlkpa. inv H2. inv H1.
-      rewrite Hlkpv in H. inv H.
-      eapply mstore_mload_same; eauto.
     
       assert (exists csa', exists c', [c] ++ csa = csa' ++ [c']) as EQ. 
         apply head_tail_commut.
       destruct EQ as [csa' [c' EQ]].
       simpl_env in EQ'.
       rewrite EQ in EQ'.
-      rewrite_env ((cs1 ++  [insn_store SI_id0 (PI_typ pinfo) SI_value0 
-                 (value_id (PI_id pinfo)) (PI_align pinfo)] ++ csa') ++ [c'])
-        in EQ'.
+      rewrite_env ((cs1 ++ [insn_alloca (PI_id pinfo) (PI_typ pinfo) 
+                 (PI_num pinfo) (PI_align pinfo)] ++ csa') ++ [c']) in EQ'.
       apply app_inj_tail in EQ'.
       destruct EQ' as [EQ1 EQ2]; subst.
       simpl in EQ.
@@ -862,7 +751,9 @@ Proof.
       simpl in G3.
       rewrite G3 in HeqR. congruence.
   
-    apply follow_alive_store_cons in J2; auto.
+    assert (getCmdLoc (insn_store sid t v1 v2 align0) <> PI_id pinfo) as Hneq.
+      admit. (* uniqness *)
+    apply follow_alive_alloca_cons in J2; auto.
     apply Hinscope in J2; auto. simpl in J2.
     destruct (fdef_dec (PI_f pinfo) (PI_f pinfo)); try congruence.
     intros gvsa gvsv Hlkpa Hlkpv.
@@ -872,15 +763,16 @@ Proof.
         apply store_notin_cmd__wf_use_at_head in HeqR; auto.
 Qed.
 
+(* its proof is same to alive_store.v *)
 Lemma mstore_preserves_wf_EC_in_tail : forall pinfo td M EC M'
   maxb gl (Hwfg: wf_globals maxb gl) lc v1 v2 gvs1 gv1 mps2 mp2 align0 t
   (H : Opsem.getOperandValue td v1 lc gl = ret gvs1)
   (H0 : Opsem.getOperandValue td v2 lc gl = ret mps2)
   (H1 : gv1 @ gvs1) (H2 : mp2 @ mps2)
-  (H3 : mstore td M mp2 t gv1 align0 = ret M') stinfo 
-  (Hinscope : wf_ExecutionContext pinfo stinfo td M gl EC)
+  (H3 : mstore td M mp2 t gv1 align0 = ret M') alinfo 
+  (Hinscope : wf_ExecutionContext pinfo alinfo td M gl EC)
   (Hht : wf_ECStack_head_in_tail maxb pinfo td M lc EC),
-  wf_ExecutionContext pinfo stinfo td M' gl EC.
+  wf_ExecutionContext pinfo alinfo td M' gl EC.
 Proof.
   intros.
   intros J1 J2 J3. 
@@ -891,16 +783,17 @@ Proof.
     eapply operand__no_alias_with__tail; eauto.
 Qed.
 
+(* its proof is same to alive_store.v *)
 Lemma mstore_preserves_wf_ECStack_in_tail : forall maxb pinfo td M  
   (Hwfpi: WF_PhiInfo pinfo) M' gl (Hwfg: wf_globals maxb gl)
   maxb gl (Hwfg: wf_globals maxb gl) lc v1 v2 gvs1 gv1 mps2 mp2 align0 t
   (H : Opsem.getOperandValue td v1 lc gl = ret gvs1)
   (H0 : Opsem.getOperandValue td v2 lc gl = ret mps2)
   (H1 : gv1 @ gvs1) (H2 : mp2 @ mps2)
-  (H3 : mstore td M mp2 t gv1 align0 = ret M') stinfo ECs 
+  (H3 : mstore td M mp2 t gv1 align0 = ret M') alinfo ECs 
   (Hhts: wf_ECStack_head_tail maxb pinfo td M lc ECs)
-  (Hwf: wf_ECStack pinfo stinfo td M gl ECs),
-  wf_ECStack pinfo stinfo td M' gl ECs.
+  (Hwf: wf_ECStack pinfo alinfo td M gl ECs),
+  wf_ECStack pinfo alinfo td M' gl ECs.
 Proof.
   induction ECs; simpl; intros; auto.
     destruct Hwf as [J1 J2].
@@ -911,6 +804,7 @@ Proof.
         in H3; eauto.
 Qed.
 
+(* same to alive_store.v *)
 Ltac preservation_malloc :=
   destruct_ctx_other;
   split; simpl; try solve [
@@ -931,10 +825,10 @@ Proof.
 Qed.
 
 Lemma callExternalFunction_preserves_wf_EC_in_tail : forall pinfo td M EC M' gl
-  stinfo gvs fid oresult
+  alinfo gvs fid oresult
   (Hcall: OpsemAux.callExternalFunction M fid gvs = ret (oresult, M'))
-  (Hinscope : wf_ExecutionContext pinfo stinfo td M gl EC),
-  wf_ExecutionContext pinfo stinfo td M' gl EC.
+  (Hinscope : wf_ExecutionContext pinfo alinfo td M gl EC),
+  wf_ExecutionContext pinfo alinfo td M' gl EC.
 Proof.
   intros.
   intros J1 J2 J3. 
@@ -945,10 +839,10 @@ Proof.
 Qed.
 
 Lemma callExternalFunction_preserves_wf_ECStack_in_tail: forall Mem fid gvs 
-  oresult Mem' pinfo stinfo TD gl ECs,
+  oresult Mem' pinfo alinfo TD gl ECs,
   OpsemAux.callExternalFunction Mem fid gvs = ret (oresult, Mem') ->
-  wf_ECStack pinfo stinfo TD Mem gl ECs ->
-  wf_ECStack pinfo stinfo TD Mem' gl ECs.
+  wf_ECStack pinfo alinfo TD Mem gl ECs ->
+  wf_ECStack pinfo alinfo TD Mem' gl ECs.
 Proof.
   induction ECs; simpl; intros; auto.
     destruct H0.
@@ -957,14 +851,14 @@ Proof.
 Qed.
 
 Lemma callExternalFunction_preserves_wf_ECStack_at_head: forall Mem fid gvs 
-  oresult Mem' pinfo stinfo gl rid noret0 ca ft fv lp cs lc lc' als tmn
+  oresult Mem' pinfo alinfo gl rid noret0 ca ft fv lp cs lc lc' als tmn
   cs1' l1 ps1 F ifs s los nts Ps (Hwfpi : WF_PhiInfo pinfo)
   (HwfF: wf_fdef ifs s (module_intro los nts Ps) F) (HuniqF: uniqFdef F)
   (H4 : OpsemAux.callExternalFunction Mem fid gvs = ret (oresult, Mem'))
   (H5 : Opsem.exCallUpdateLocals (los,nts) ft noret0 rid oresult lc = ret lc')
-  (HBinF : blockInFdefB (block_intro l1 ps1 (cs1' ++ insn_call rid noret0 ca ft fv lp :: cs) tmn)
-             F = true)
-  (Hinscope : wf_ExecutionContext pinfo stinfo (los,nts) Mem gl
+  (HBinF : blockInFdefB (block_intro l1 ps1 (cs1' ++ insn_call rid noret0 ca ft fv lp :: cs) 
+             tmn) F = true)
+  (Hinscope : wf_ExecutionContext pinfo alinfo (los,nts) Mem gl
                {|
                Opsem.CurFunction := F;
                Opsem.CurBB := block_intro l1 ps1
@@ -974,7 +868,7 @@ Lemma callExternalFunction_preserves_wf_ECStack_at_head: forall Mem fid gvs
                Opsem.Terminator := tmn;
                Opsem.Locals := lc;
                Opsem.Allocas := als |}),
-   wf_ExecutionContext pinfo stinfo (los,nts) Mem' gl
+   wf_ExecutionContext pinfo alinfo (los,nts) Mem' gl
      {|
      Opsem.CurFunction := F;
      Opsem.CurBB := block_intro l1 ps1
@@ -987,7 +881,9 @@ Proof.
   intros.
   intros J1 J2 J3. simpl in J1, J2, J3. simpl. subst.
   assert (J2':=J2).
-  apply follow_alive_store_cons in J2; auto.
+  assert (rid <> PI_id pinfo) as Hneq. 
+    eapply WF_PhiInfo_spec10 in HBinF; eauto.
+  apply follow_alive_alloca_cons in J2; auto.
   apply Hinscope in J2; auto. 
   simpl in J2.
   intros gvsa gvsv Hlka Hlkv.
@@ -1001,26 +897,20 @@ Proof.
     destruct ft; tinv H0.
     remember (fit_gv (los,nts) ft g) as R.
     destruct R; inv H0.
-    assert (rid <> PI_id pinfo) as Hneq. 
-      eapply WF_PhiInfo_spec10 in HBinF; eauto.
     rewrite <- lookupAL_updateAddAL_neq in Hlka; auto.
-    assert (used_in_value rid (SI_value pinfo stinfo) = false) as Hnouse.
-      eapply alive_store_doesnt_use_its_followers; eauto 
-        using wf_system__wf_fdef, follow_alive_store_cons.
     apply getOperandValue_updateAddAL_nouse in Hlkv; auto.
     eapply MemProps.callExternalFunction_preserves_mload; eauto.
 Qed.
 
+Ltac WF_PhiInfo_spec10_tac :=
+  match goal with
+  | HBinF1 : blockInFdefB (block_intro _ _ (_ ++ _ :: _) _) _ = true |- _ =>
+     eapply WF_PhiInfo_spec10 in HBinF1; eauto using wf_system__uniqFdef
+  end.
+
 Ltac preservation_pure_cmd_updated_case_helper:=
   destruct_ctx_other;
-  intros; subst;
-  split; try 
-  eapply alive_store_doesnt_use_its_followers; try solve [
-    eauto using wf_system__wf_fdef |
-    match goal with
-    | HBinF1 : blockInFdefB (block_intro _ _ (_ ++ _ :: _) _) _ = true |- _ =>
-       eapply WF_PhiInfo_spec10 in HBinF1; eauto using wf_system__uniqFdef
-    end].
+  intros; subst; WF_PhiInfo_spec10_tac.
 
 Ltac preservation_pure_cmd_updated_case:=
   abstract (eapply preservation_pure_cmd_updated_case; eauto; try solve
@@ -1031,7 +921,8 @@ match goal with
 | Hinscope: wf_ExecutionContext ?pinfo _ _ _ _ _ |- _ =>
   intros J1 J2 J3; simpl in J1, J2, J3; simpl; subst;
   assert (J2':=J2);
-  apply follow_alive_store_cons in J2; eauto using wf_system__uniqFdef;
+  apply follow_alive_alloca_cons in J2; eauto using wf_system__uniqFdef;
+    try solve [WF_PhiInfo_spec10_tac];
   apply Hinscope in J2; auto; simpl in J2;
   destruct (fdef_dec (PI_f pinfo) (PI_f pinfo)); try congruence;
   intros gvsa gvsv Hlkpa Hlkpv;
@@ -1043,12 +934,12 @@ match goal with
     ]
 end.
 
-Lemma preservation : forall maxb pinfo stinfo cfg S1 S2 tr
+Lemma preservation : forall maxb pinfo alinfo cfg S1 S2 tr
   (Hwfg: wf_globals maxb (OpsemAux.Globals cfg))
   (Hwfpp: OpsemPP.wf_State cfg S1) 
   (Hnoalias: Promotability.wf_State maxb pinfo cfg S1) 
   (HwfPI: WF_PhiInfo pinfo) (HsInsn: Opsem.sInsn cfg S1 S2 tr)
-  (HwfS1: wf_State pinfo stinfo cfg S1), wf_State pinfo stinfo cfg S2.
+  (HwfS1: wf_State pinfo alinfo cfg S1), wf_State pinfo alinfo cfg S2.
 Proof.
   intros.
   (sInsn_cases (induction HsInsn) Case); destruct TD as [los nts]; simpl HwfS1.
@@ -1101,7 +992,7 @@ Case "sCall".
   destruct_ctx_other;
   split; try solve [
     intros J1 J2 J3; simpl in J1, J2, J3; simpl;
-    eapply follow_alive_store_at_beginning_false in J2; eauto; inv J2 |
+    eapply follow_alive_alloca_at_beginning_false in J2; eauto; inv J2 |
     split; auto]).
 
 Case "sExCall". 
@@ -1113,10 +1004,10 @@ Case "sExCall".
     eapply callExternalFunction_preserves_wf_ECStack_in_tail; eauto]).
 Qed.
 
-Lemma s_genInitState__alive_store: forall S main VarArgs cfg IS pinfo stinfo
+Lemma s_genInitState__alive_alloca: forall S main VarArgs cfg IS pinfo alinfo
   (HwfS : wf_system nil S) (Hwfpi: WF_PhiInfo pinfo) 
   (Hinit : @Opsem.s_genInitState DGVs S main VarArgs Mem.empty = ret (cfg, IS)),
-  wf_State pinfo stinfo cfg IS.
+  wf_State pinfo alinfo cfg IS.
 Admitted.
  
 (*****************************)
