src/Transforms/sas.v
@@ -19,6 +19,7 @@ Require Import palloca_props.
 Require Import memory_props.
 Require Import mem2reg.
 Require Import program_sim.
+Require Import trans_tactic.
 
 Definition sas (sid1 sid2: id) (v1 v2:value) (cs2:cmds) (b:block) 
   (pinfo:PhiInfo) : Prop :=         
@@ -131,8 +132,7 @@ Definition undead_head_in_tail (pinfo:PhiInfo) (sasinfo: SASInfo pinfo) ptr
   (ec0:@Opsem.ExecutionContext DGVs) : Prop :=
 forall gvsa (Heq: Opsem.CurFunction ec0 = PI_f pinfo)
   (Hlkup: lookupAL _ (Opsem.Locals ec0) (PI_id pinfo) = Some gvsa),
-  MemProps.no_alias ptr gvsa \/
-  ~ MemProps.no_alias ptr gvsa /\ EC_follow_dead_store pinfo sasinfo ec0.
+  MemProps.no_alias ptr gvsa \/ ~ EC_follow_dead_store pinfo sasinfo ec0.
 
 Definition undead_head_tail (pinfo:PhiInfo) (sasinfo: SASInfo pinfo) ptr 
   (ecs':list Opsem.ExecutionContext) : Prop :=
@@ -186,6 +186,473 @@ Proof.
   destruct (id_dec i0 (SAS_sid1 pinfo sasinfo)); auto.
 Qed.
 
+Ltac repeat_solve :=
+  repeat (match goal with
+          | |- Mem_simulation _ _ _ _ _ _ => idtac 
+          | |- _ => split; eauto 2 using cmds_at_block_tail_next
+          end).
+
+Lemma mstore_removable_Mem_simulation: forall TD M1 mp2 gv1 a M1' pinfo lc2 gl2
+  B1 cs1 tmn2 als2 ECs1 M2 t v sasinfo v0
+  (Huniq: uniqFdef (PI_f pinfo))
+  (HBinF1 : blockInFdefB B1 (PI_f pinfo) = true)
+  (Heq3 : exists l1 : l,
+           exists ps1 : phinodes,
+             exists cs11 : list cmd,
+               B1 =
+               block_intro l1 ps1
+                 (cs11 ++ insn_store (SAS_sid1 pinfo sasinfo) t v v0 a :: cs1)
+                 tmn2)
+  (H23: mstore TD M1 mp2 t gv1 a = ret M1')
+  (H20 : @Opsem.getOperandValue DGVs TD v0 lc2 gl2 = ret mp2)
+  (H19 : Opsem.getOperandValue TD v lc2 gl2 = ret gv1)
+  (Hmsim: Mem_simulation pinfo sasinfo TD
+            ({|
+             Opsem.CurFunction := PI_f pinfo;
+             Opsem.CurBB := B1;
+             Opsem.CurCmds := insn_store (SAS_sid1 pinfo sasinfo) t v v0 a
+                              :: cs1;
+             Opsem.Terminator := tmn2;
+             Opsem.Locals := lc2;
+             Opsem.Allocas := als2 |} :: ECs1) M1 M2),
+  Mem_simulation pinfo sasinfo TD
+            ({|
+             Opsem.CurFunction := PI_f pinfo;
+             Opsem.CurBB := B1;
+             Opsem.CurCmds := cs1;
+             Opsem.Terminator := tmn2;
+             Opsem.Locals := lc2;
+             Opsem.Allocas := als2 |} :: ECs1) M1' M2.
+Proof.
+  intros.
+  destruct Hmsim as [Hmsim1 Hmsim2].
+  split.
+    apply MemProps.nextblock_mstore in H23.
+    rewrite <- H23. auto.
+
+    intros. 
+    assert (In {|
+               Opsem.CurFunction := PI_f pinfo;
+               Opsem.CurBB := B1;
+               Opsem.CurCmds := cs1;
+               Opsem.Terminator := tmn2;
+               Opsem.Locals := lc2;
+               Opsem.Allocas := als2 |}
+              ({|
+               Opsem.CurFunction := PI_f pinfo;
+               Opsem.CurBB := B1;
+               Opsem.CurCmds := cs1;
+               Opsem.Terminator := tmn2;
+               Opsem.Locals := lc2;
+               Opsem.Allocas := als2 |} :: ECs1)) as Hin. simpl. auto.
+    apply Hnalias in Hin. 
+    unfold undead_head_in_tail in Hin. simpl in Hin.
+    assert (v0 = value_id (PI_id pinfo)) as EQ.
+      admit. (* uniqness *)
+    subst. simpl in H20.
+    assert (Hlkup:=H20).
+    apply Hin in H20; auto.
+    destruct H20 as [Hnalias' | Hnfollow].
+      eapply Hmsim2; eauto.
+        unfold undead_head_tail. intros.
+        simpl in Hin0.
+        destruct Hin0 as [Hin0 | Hin0]; subst.
+          unfold undead_head_in_tail. simpl.
+          intros. rewrite Hlkup in Hlkup0. inv Hlkup0. auto.
+
+          apply Hnalias. simpl. auto.
+
+        apply MemProps.no_alias_sym in Hnalias'.
+        eapply MemProps.mstore_preserves_mload_inv'; eauto.
+
+      contradict Hnfollow.
+      destruct Heq3 as [l1 [ps1 [cs11 Heq3]]]; subst.
+      split; auto. simpl.
+      assert (block_intro l1 ps1
+               (cs11 ++
+                insn_store (SAS_sid1 pinfo sasinfo) t v (value_id (PI_id pinfo)) 
+                  a :: cs1) tmn2 = SAS_block pinfo sasinfo) as EQ.
+        admit. (* uniqness *)
+      split; auto.
+        unfold cs_follow_dead_store.
+        rewrite <- EQ.
+        clear - HBinF1.
+        intros.
+        assert (cs11 = cs0 /\ cs1 = SAS_tail pinfo sasinfo ++ cs3 /\
+                t = PI_typ pinfo /\ v = SAS_value1 pinfo sasinfo /\
+                a = PI_align pinfo) as EQ.
+          admit.
+        destruct EQ as [EQ1 [EQ2 [EQ3 [EQ4 EQ5]]]]; subst.
+        exists nil. exists (SAS_tail pinfo sasinfo). auto.
+Qed.
+
+Lemma cmds_simulation_elim_cons_inv: forall (pinfo : PhiInfo) sasinfo
+  (t : typ) (v1 v2: value) (a : align) (cs1 : list cmd) (cs2 : cmds)
+  (Hcssim2 : 
+   cmds_simulation pinfo sasinfo (PI_f pinfo)
+     (insn_store (SAS_sid1 pinfo sasinfo) t v1 v2 a :: cs1)
+     cs2),
+  cmds_simulation pinfo sasinfo (PI_f pinfo) cs1 cs2.
+Proof.
+  intros.
+  unfold cmds_simulation in *.
+  destruct (fdef_dec (PI_f pinfo) (PI_f pinfo)); try congruence.
+  simpl in *.
+  destruct (id_dec (SAS_sid1 pinfo sasinfo) (SAS_sid1 pinfo sasinfo)); 
+    simpl in *; try congruence.
+Qed.
+
+
+Lemma cmds_simulation_nil_inv: forall pinfo sasinfo f1 cs,
+  cmds_simulation pinfo sasinfo f1 nil cs -> cs = nil.
+Proof.
+  unfold cmds_simulation. simpl.
+  intros. destruct (fdef_dec (PI_f pinfo) f1); auto.
+Qed.
+
+Lemma cmds_simulation_nelim_cons_inv: forall pinfo sasinfo F c cs2 cs',
+  cmds_simulation pinfo sasinfo F (c :: cs2) cs' ->
+  (PI_f pinfo = F -> getCmdLoc c <> SAS_sid1 pinfo sasinfo) ->
+  exists cs2', 
+    cs' = c :: cs2' /\ cmds_simulation pinfo sasinfo F cs2 cs2'.
+Proof.  
+  intros.
+  unfold cmds_simulation in *.
+  destruct (fdef_dec (PI_f pinfo) F); subst; simpl; eauto.
+  assert (PI_f pinfo = PI_f pinfo) as EQ. auto.
+  apply H0 in EQ.
+  destruct (id_dec (getCmdLoc c) (SAS_sid1 pinfo sasinfo)); 
+    simpl in *; try congruence.
+  eauto.
+Qed.
+
+Ltac destruct_ctx_return :=
+match goal with
+| Hwfpp : OpsemPP.wf_State
+            {|
+            OpsemAux.CurSystem := _;
+            OpsemAux.CurTargetData := ?TD;
+            OpsemAux.CurProducts := _;
+            OpsemAux.Globals := _;
+            OpsemAux.FunTable := _
+             |} _,
+  Hnoalias : Promotability.wf_State _ _ _ _,
+  Hsim : State_simulation _ _ _ _ ?Cfg2 ?St2 ,
+  Hop2 : Opsem.sInsn _ _ _ _ |- _ =>
+  destruct TD as [los nts];
+  destruct Hwfpp as 
+    [Hwfg [HwfSystem [HmInS [_ [
+     [Hreach1 [HBinF1 [HFinPs1 _]]] 
+     [ 
+       [
+         [Hreach2 [HBinF2 [HFinPs2 _]]]
+         _
+       ]
+       HwfCall'
+     ]]
+    ]]]]; subst;
+  destruct Cfg2 as [S2 TD2 Ps2 gl2 fs2];
+  destruct St2 as [ECs2 M2];
+  simpl in Hsim;
+  destruct Hsim as [EQ1 [Hpsim [Hstksim [EQ2 [EQ3 Hmsim]]]]]; subst;
+  destruct ECs2 as [|[F2 B2 cs2 tmn2 lc2 als2] ECs2]; tinv Hstksim;
+  destruct Hstksim as [Hecsim Hstksim];
+  destruct ECs2 as [|[F3 B3 cs3 tmn3 lc3 als3] ECs2]; tinv Hstksim;
+  destruct Hstksim as [Hecsim' Hstksim];
+  unfold EC_simulation in Hecsim;
+  destruct Hecsim as 
+      [Hfsim2 [Heq1 [Heq2 [Hbsim2 
+        [Heq3 [Heq4 [Hlcsim2 Hcssim2]]]]]]]; subst;
+  destruct Hecsim' as 
+      [Hfsim2' [Htsim2' [Heq2' [Hbsim2' 
+        [Heq3' [Heq4' [Hlcsim2' Hcssim2']]]]]]]; subst;
+  destruct Hnoalias as 
+    [
+      [[Hinscope1' _] [[[Hinscope2' _] [HwfECs' _]] _]] 
+      [[Hdisjals _] HwfM]
+    ]; simpl in Hdisjals;
+  fold Promotability.wf_ECStack in HwfECs';
+  apply cmds_simulation_nil_inv in Hcssim2; subst;
+  wfCall_inv;
+  apply cmds_simulation_nelim_cons_inv in Hcssim2'; try solve [
+    auto |
+    try match goal with
+        | |- _ = _ -> _ <> _ => admit
+        end ];
+  destruct Hcssim2' as [cs3' [Heq Hcssim2']]; subst;
+  inv Hop2;
+  uniq_result
+end.
+
+
+Lemma cs_follow_dead_store_isnt_nil: forall pinfo sasinfo,
+  cs_follow_dead_store pinfo sasinfo nil -> False.
+Proof.
+  intros.
+  unfold cs_follow_dead_store in H.
+  destruct sasinfo. simpl in *.
+  destruct SAS_block0.
+  destruct SAS_prop0 as [J1 [J4 [cs1 [cs2 EQ]]]].
+  apply H in EQ.
+  destruct EQ as [csa [csb [EQ1 EQ2]]].
+  symmetry in EQ1.
+  apply app_eq_nil in EQ1. destruct EQ1 as [EQ11 EQ12]. inv EQ12.
+Qed.
+
+Lemma undead_head_in_tail_nil: forall pinfo sasinfo ptr F B tmn lc als,
+  undead_head_in_tail pinfo sasinfo ptr
+    {| Opsem.CurFunction := F;
+       Opsem.CurBB := B;
+       Opsem.CurCmds := nil;
+       Opsem.Terminator := tmn;
+       Opsem.Locals := lc;
+       Opsem.Allocas := als |}.
+Proof.
+  intros.
+  unfold undead_head_in_tail. simpl. intros.
+  right. intros [J1 [J2 J3]]. simpl in J1, J2, J3.
+  eapply cs_follow_dead_store_isnt_nil; eauto.
+Qed.
+
+Lemma cs_follow_dead_store_tail: forall pinfo sasinfo c cs,
+  getCmdLoc c <> SAS_sid2 pinfo sasinfo ->
+  cs_follow_dead_store pinfo sasinfo (c :: cs) ->
+  cs_follow_dead_store pinfo sasinfo cs.
+Proof.
+  unfold cs_follow_dead_store.
+  destruct sasinfo. simpl. intros.
+  destruct SAS_block0.
+  intros. 
+  destruct SAS_prop0 as [EQ1 [EQ2 [cs4 [cs2 EQ3]]]]; subst.
+  assert (cs4 = cs1 /\ 
+          cs3 = insn_store SAS_sid4 (PI_typ pinfo) SAS_value4
+                  (value_id (PI_id pinfo)) (PI_align pinfo) :: cs2) as EQ.
+    admit. 
+  destruct EQ as [EQ3 EQ4]; subst.
+  edestruct H0 as [csa [csb [J1 J2]]]; subst; eauto.
+  destruct csb.
+    inv J1. contradict H; auto.
+
+    inv J1. exists (csa++[c0]). exists csb. simpl_env. split; auto.
+Qed.
+
+Lemma EC_follow_dead_store_tail: forall pinfo sasinfo c cs B tmn3 lc1 als3 lc2 F,
+  getCmdLoc c <> SAS_sid2 pinfo sasinfo ->
+  ~ EC_follow_dead_store pinfo sasinfo
+      {| Opsem.CurFunction := F;
+         Opsem.CurBB := B;
+         Opsem.CurCmds := cs;
+         Opsem.Terminator := tmn3;
+         Opsem.Locals := lc1;
+         Opsem.Allocas := als3 |} ->
+  ~ EC_follow_dead_store pinfo sasinfo
+      {| Opsem.CurFunction := F;
+         Opsem.CurBB := B;
+         Opsem.CurCmds := c :: cs;
+         Opsem.Terminator := tmn3;
+         Opsem.Locals := lc2;
+         Opsem.Allocas := als3 |}.
+Proof.
+  intros.
+  intro J. apply H0.
+  destruct J as [J1 [J2 J3]]. simpl in *.
+  split; auto.
+  split; auto.
+    simpl. 
+    eapply cs_follow_dead_store_tail; eauto.
+Qed.
+
+Lemma cs_follow_dead_store_at_beginning_false: forall (pinfo : PhiInfo) 
+  (sasinfo : SASInfo pinfo) (l' : l) (ps' : phinodes) (cs' : cmds) 
+  (tmn' : terminator) 
+  (J2 : block_intro l' ps' cs' tmn' = SAS_block pinfo sasinfo)
+  (J3 : cs_follow_dead_store pinfo sasinfo cs'),
+  False.
+Proof.
+  intros.
+  unfold cs_follow_dead_store in J3.
+  rewrite <- J2 in J3.
+  destruct sasinfo. simpl in *.
+  rewrite <- J2 in SAS_prop0.
+  destruct SAS_prop0 as [_ [_ [cs1 [cs3 J]]]].
+  assert (J':=J).
+  apply J3 in J.
+  destruct J as [csa [csb [EQ1 EQ2]]]; subst.
+  rewrite_env (
+    (cs1 ++
+     insn_store SAS_sid3 (PI_typ pinfo) SAS_value3 
+         (value_id (PI_id pinfo)) (PI_align pinfo) :: (csa ++ csb)) ++ 
+     insn_store SAS_sid4 (PI_typ pinfo) SAS_value4
+            (value_id (PI_id pinfo)) (PI_align pinfo) :: cs3
+    ) in J'.
+  apply app_inv_tail in J'. 
+  rewrite_env (nil ++ csb) in J'.
+  rewrite_env (
+    (cs1 ++
+       insn_store SAS_sid3 (PI_typ pinfo) SAS_value3 
+         (value_id (PI_id pinfo)) (PI_align pinfo) :: 
+       csa) ++ csb
+    ) in J'.
+  apply app_inv_tail in J'. 
+  assert (
+    In (insn_store SAS_sid3 (PI_typ pinfo) SAS_value3 
+         (value_id (PI_id pinfo)) (PI_align pinfo)) nil) as Hin.
+    rewrite J'. apply in_middle.
+  inv Hin.
+Qed.
+
+Lemma cs_follow_dead_store_at_end_false: forall (pinfo : PhiInfo) 
+  (sasinfo : SASInfo pinfo) (J3 : cs_follow_dead_store pinfo sasinfo nil),
+  False.
+Proof.
+  intros.
+  unfold cs_follow_dead_store in J3.
+  destruct sasinfo. simpl in *. destruct SAS_block0.
+  destruct SAS_prop0 as [_ [_ [cs1 [cs3 J]]]].
+  assert (J':=J).
+  apply J3 in J.
+  destruct J as [csa [csb [EQ1 EQ2]]]; subst.
+  assert (
+    In (insn_store SAS_sid4 (PI_typ pinfo) SAS_value4 
+         (value_id (PI_id pinfo)) (PI_align pinfo)) nil) as Hin.
+    rewrite EQ1. apply in_middle.
+  inv Hin.
+Qed.
+
+Lemma EC_follow_dead_store_at_end_false: forall pinfo sasinfo F B tmn lc2 als2,
+   ~
+   EC_follow_dead_store pinfo sasinfo
+     {|
+     Opsem.CurFunction := F;
+     Opsem.CurBB := B;
+     Opsem.CurCmds := nil;
+     Opsem.Terminator := tmn;
+     Opsem.Locals := lc2;
+     Opsem.Allocas := als2 |}.
+Proof.
+  intros. intro J.
+  destruct J as [J1 [J2 J3]]. simpl in *.
+  eapply cs_follow_dead_store_at_end_false in J3; eauto.  
+Qed.
+
+Ltac destruct_ctx_other :=
+match goal with
+| Hwfpp : OpsemPP.wf_State
+            {|
+            OpsemAux.CurSystem := _;
+            OpsemAux.CurTargetData := ?TD;
+            OpsemAux.CurProducts := _;
+            OpsemAux.Globals := _;
+            OpsemAux.FunTable := _
+             |} _,
+  Hnoalias : Promotability.wf_State _ _ _ _,
+  Hsim : State_simulation _ _ _ _ ?Cfg2 ?St2 ,
+  Hop2 : Opsem.sInsn _ _ _ _ |- _ =>
+  destruct TD as [los nts];
+  destruct Hwfpp as 
+    [Hwfg [HwfSystem [HmInS [_ [
+     [Hreach1 [HBinF1 [HFinPs1 _]]] 
+     [ _ HwfCall'
+     ]]
+    ]]]]; subst;
+  destruct Cfg2 as [S2 TD2 Ps2 gl2 fs2];
+  destruct St2 as [ECs2 M2];
+  simpl in Hsim;
+  destruct Hsim as [EQ1 [Hpsim [Hstksim [EQ2 [EQ3 Hmsim]]]]]; subst;
+  destruct ECs2 as [|[F2 B2 cs2 tmn2 lc2 als2] ECs2]; tinv Hstksim;
+  destruct Hstksim as [Hecsim Hstksim];
+  unfold EC_simulation in Hecsim;
+  destruct Hecsim as 
+      [Hfsim2 [Heq1 [Heq2 [Hbsim2 
+        [Heq3 [Heq4 [Hlcsim2 Hcssim2]]]]]]]; subst;
+  destruct Hnoalias as 
+    [
+      [[Hinscope' _] [HwfECs' HwfHT]] 
+      [[Hdisjals _] HwfM]
+    ]; simpl in Hdisjals;
+  fold Promotability.wf_ECStack in HwfECs'
+end.
+
+Lemma fdef_sim__block_sim : forall pinfo sasinfo f1 f2 b1 b2 l0,
+  fdef_simulation pinfo sasinfo f1 f2 ->
+  lookupBlockViaLabelFromFdef f1 l0 = Some b1 ->
+  lookupBlockViaLabelFromFdef f2 l0 = Some b2 ->
+  block_simulation pinfo sasinfo f1 b1 b2.
+Admitted.
+
+Lemma remove_phinodes_eq: forall pinfo sasinfo l0 ps0 cs0 tmn0,
+  WF_PhiInfo pinfo -> uniqFdef (PI_f pinfo) ->
+  blockInFdefB (block_intro l0 ps0 cs0 tmn0) (PI_f pinfo) ->
+  remove_phinodes (SAS_sid1 pinfo sasinfo) ps0 = ps0.
+Admitted.
+
+Lemma block_simulation_inv : forall pinfo sasinfo F l1 ps1 cs1 tmn1 l2 ps2 cs2
+  tmn2,
+  WF_PhiInfo pinfo -> uniqFdef F ->
+  blockInFdefB (block_intro l1 ps1 cs1 tmn1) F ->
+  block_simulation pinfo sasinfo F (block_intro l1 ps1 cs1 tmn1)
+    (block_intro l2 ps2 cs2 tmn2) ->
+  l1 = l2 /\ ps1 = ps2 /\ 
+  cmds_simulation pinfo sasinfo F cs1 cs2 /\ tmn1 = tmn2.
+Proof.
+  intros.
+  unfold block_simulation, cmds_simulation in *.
+  destruct (fdef_dec (PI_f pinfo) F); inv H2; auto.
+  erewrite remove_phinodes_eq; eauto.
+Qed.
+
+Lemma switchToNewBasicBlock_sim : forall TD l1 l2 ps cs1 cs2 tmn1 tmn2 B1 B2 
+  gl lc lc1 lc2 F pinfo sasinfo 
+  (H23 : @Opsem.switchToNewBasicBlock DGVs TD
+          (block_intro l1 ps cs1 tmn1) B1 gl lc = 
+         ret lc1)
+  (Hbsim2 : block_simulation pinfo sasinfo F B1 B2)
+  (H2 : Opsem.switchToNewBasicBlock TD
+         (block_intro l2 ps cs2 tmn2) B2 gl lc = 
+        ret lc2), lc1 = lc2.
+Admitted.
+
+Lemma switchToNewBasicBlock_Mem_simulation: forall (pinfo : PhiInfo) 
+  (sasinfo : SASInfo pinfo) (gl2 : GVMap) (lc2 : Opsem.GVsMap) 
+  (als2 : list mblock) (M2 : mem) (los : layouts) (nts : namedts) (F : fdef)
+  (B : block) tmn 
+  (EC : list Opsem.ExecutionContext) (Mem : mem) (cs' : cmds)
+  (Hmsim : Mem_simulation pinfo sasinfo (los, nts)
+            ({|
+             Opsem.CurFunction := F;
+             Opsem.CurBB := B;
+             Opsem.CurCmds := nil;
+             Opsem.Terminator := tmn;
+             Opsem.Locals := lc2;
+             Opsem.Allocas := als2 |} :: EC) Mem M2)
+  (l'0 : l) (ps'0 : phinodes) (tmn'0 : terminator) (lc'0 : Opsem.GVsMap)
+  (H2 : Opsem.switchToNewBasicBlock (los, nts)
+         (block_intro l'0 ps'0 cs' tmn'0) B gl2 lc2 = 
+        ret lc'0),
+  Mem_simulation pinfo sasinfo (los, nts)
+     ({|
+      Opsem.CurFunction := F;
+      Opsem.CurBB := block_intro l'0 ps'0 cs' tmn'0;
+      Opsem.CurCmds := cs';
+      Opsem.Terminator := tmn'0;
+      Opsem.Locals := lc'0;
+      Opsem.Allocas := als2 |} :: EC) Mem M2.
+Proof.
+  intros.
+  destruct Hmsim as [Hmsim1 Hmsim2].
+  split; auto.
+    intros.
+    eapply Hmsim2 with (ptr:=ptr)(ty:=ty)(al:=al); eauto.
+    unfold undead_head_tail in *.
+    intros.
+    simpl in Hin.
+    destruct Hin as [Hin | Hin]; subst.
+      unfold undead_head_in_tail in *. simpl in *. intros. 
+      right. apply EC_follow_dead_store_at_end_false.
+ 
+      apply Hnalias; simpl; auto.
+Qed.
+    
 Lemma sas_is_sim : forall maxb pinfo (sasinfo: SASInfo pinfo) Cfg1 St1 Cfg2 St2
   (Hwfpi: WF_PhiInfo pinfo) 
   (Hwfpp: OpsemPP.wf_State Cfg1 St1) 
@@ -198,7 +665,480 @@ Lemma sas_is_sim : forall maxb pinfo (sasinfo: SASInfo pinfo) Cfg1 St1 Cfg2 St2
      (Hop2: Opsem.sInsn Cfg2 St2 St2' tr2) 
      (Hop1: Opsem.sInsn Cfg1 St1 St1' tr1), 
      State_simulation pinfo sasinfo Cfg1 St1' Cfg2 St2' /\ tr1 = tr2).
+Proof.
+
+Local Opaque inscope_of_tmn inscope_of_cmd.
+
+  intros.
+  split; intros.
+Case "removable state".
+  
+  destruct Cfg1 as [S1 [los nts] Ps1 gl1 fs1].
+  destruct St1 as [ECs1 M1].
+  destruct ECs1 as [|[F1 B1 [|[] cs1] tmn1 lc1 als1] ECs1]; tinv Hrem.
+  simpl in Hrem.
+  destruct (fdef_dec (PI_f pinfo) F1); subst; tinv Hrem.
+  destruct (id_dec i0 (SAS_sid1 pinfo sasinfo)); subst; tinv Hrem.
+  
+  destruct Hwfpp as 
+    [Hwfg [HwfSystem [HmInS [_ [
+     [Hreach1 [HBinF1 [HFinPs1 _]]] 
+     [HwfECs Hwfcall]]
+    ]]]]; subst.
+  fold (@OpsemPP.wf_ECStack DGVs) in HwfECs.
+
+  destruct Hnoalias as 
+    [
+      [[Hinscope' _] [HwfECs' HwfHT]] 
+      [[Hdisjals _] HwfM]
+    ]; simpl in Hdisjals.
+  fold Promotability.wf_ECStack in HwfECs'.
+
+  inv Hop1.
+
+  destruct Cfg2 as [S2 TD2 Ps2 gl2 fs2].
+  destruct St2 as [ECs2 M2].
+
+  simpl in Hsim.
+  destruct Hsim as [EQ1 [Hpsim [Hstksim [EQ2 [EQ3 Hmsim]]]]]; subst.
+  destruct ECs2 as [|[F2 B2 cs2 tmn2 lc2 als2] ECs2]; tinv Hstksim.
+  destruct Hstksim as [Hecsim Hstksim].
+  unfold EC_simulation in Hecsim.
+  destruct Hecsim as 
+      [Hfsim2 [Heq1 [Heq2 [Hbsim2 
+        [Heq3 [Heq4 [Hlcsim2 Hcssim2]]]]]]]; subst.
+
+  uniq_result.
+  repeat_solve.
+    eapply cmds_simulation_elim_cons_inv; eauto.
+    eapply mstore_removable_Mem_simulation in Hmsim; 
+      eauto using wf_system__uniqFdef.
+
+Case "unremovable state".
+  (sInsn_cases (destruct Hop1) SCase).
+
+SCase "sReturn".
+Focus.
+  destruct_ctx_return.
+  repeat_solve.
+
+    clear - H26 Hmsim H0 H1 Hinscope1' HBinF2 Heq3'.
+    destruct Hmsim as [Hmsim1 Hmsim2].
+    split.
+      apply MemProps.nextblock_free_allocas in H0.
+      apply MemProps.nextblock_free_allocas in H26.
+      rewrite <- H0. rewrite <- H26. auto.
+
+      intros.
+      eapply Hmsim2 with (ptr:=ptr)(ty:=ty)(al:=al);
+        eauto using MemProps.free_allocas_preserves_mload_inv.
+      unfold undead_head_tail. simpl.
+      intros.
+      destruct Hin as [Hin | [Hin | Hin]]; subst.
+        apply undead_head_in_tail_nil.
+
+        unfold undead_head_in_tail. simpl.
+        assert (In {| Opsem.CurFunction := F';
+                      Opsem.CurBB := B';
+                      Opsem.CurCmds := cs';
+                      Opsem.Terminator := tmn3;
+                      Opsem.Locals := lc''0;
+                      Opsem.Allocas := als3 |}
+                   ({| Opsem.CurFunction := F';
+                       Opsem.CurBB := B';
+                       Opsem.CurCmds := cs';
+                       Opsem.Terminator := tmn3;
+                       Opsem.Locals := lc''0;
+                       Opsem.Allocas := als3 |} :: EC)) as Hin.
+          simpl. auto.
+        apply Hnalias in Hin.
+        unfold undead_head_in_tail in Hin. simpl in Hin.
+        intros. subst.
+        assert (lookupAL (GVsT DGVs) lc''0 (PI_id pinfo) = ret gvsa) as Hlkup'.
+          admit. (* rid <> pid *)
+        apply Hin in Hlkup'; auto.
+        destruct Hlkup' as [Hlkup' | Hlkup']; auto.
+        right.
+        eapply EC_follow_dead_store_tail; eauto.
+          admit. (* uniqness *)
+
+        apply Hnalias; simpl; auto.     
+Unfocus.
+      
+SCase "sReturnVoid".
+Focus.
+  destruct_ctx_return.
+  repeat_solve.
+
+    clear - H24 Hmsim H0 Hinscope1'.
+    destruct Hmsim as [Hmsim1 Hmsim2].
+    split.
+      apply MemProps.nextblock_free_allocas in H0.
+      apply MemProps.nextblock_free_allocas in H24.
+      rewrite <- H0. rewrite <- H24. auto.
+
+      intros.
+      eapply Hmsim2 with (ptr:=ptr)(ty:=ty)(al:=al);
+        eauto using MemProps.free_allocas_preserves_mload_inv.
+      unfold undead_head_tail. simpl.
+      intros.
+      destruct Hin as [Hin | [Hin | Hin]]; subst.
+        apply undead_head_in_tail_nil.
+
+        unfold undead_head_in_tail. simpl.
+        assert (In {| Opsem.CurFunction := F';
+                      Opsem.CurBB := B';
+                      Opsem.CurCmds := cs';
+                      Opsem.Terminator := tmn3;
+                      Opsem.Locals := lc3;
+                      Opsem.Allocas := als3 |}
+                   ({| Opsem.CurFunction := F';
+                       Opsem.CurBB := B';
+                       Opsem.CurCmds := cs';
+                       Opsem.Terminator := tmn3;
+                       Opsem.Locals := lc3;
+                       Opsem.Allocas := als3 |} :: EC)) as Hin.
+          simpl. auto.
+        apply Hnalias in Hin.
+        unfold undead_head_in_tail in Hin. simpl in Hin.
+        intros. subst.
+        apply Hin in Hlkup; auto.
+        destruct Hlkup as [Hlkup | Hlkup]; auto.
+        right.
+        eapply EC_follow_dead_store_tail; eauto.
+          admit. (* uniqness *)
+
+        apply Hnalias; simpl; auto.     
+Unfocus.
+
+SCase "sBranch".
+Focus.
+
+  destruct_ctx_other.
+  apply cmds_simulation_nil_inv in Hcssim2; subst.
+  inv Hop2.
+  uniq_result.
+
+  assert (block_simulation pinfo sasinfo F (block_intro l' ps' cs' tmn')
+           (block_intro l'0 ps'0 cs'0 tmn'0)) as Hbsim.
+    clear - H22 H1 Hfsim2.
+    destruct (isGVZero (los, nts) c); eauto using fdef_sim__block_sim.  
+  assert (uniqFdef F) as Huniq. eauto using wf_system__uniqFdef.
+  assert (blockInFdefB (block_intro l' ps' cs' tmn') F) as HBinF1'.
+    admit.
+  assert (Hbsim':=Hbsim).
+  apply block_simulation_inv in Hbsim'; auto.
+  destruct Hbsim' as [Heq1 [Heq2 [Hcssim' Heq5]]]; subst.
+
+  assert (lc' = lc'0) as Heq.
+    clear - H2 H23 Hbsim2.
+    eapply switchToNewBasicBlock_sim in Hbsim2; eauto.
+  subst.
+
+  repeat_solve.
+    exists l'0. exists ps'0. exists nil. auto.
+    exists l'0. exists ps'0. exists nil. auto.
+  
+    clear - H2 Hmsim.
+    eapply switchToNewBasicBlock_Mem_simulation; eauto.
+
+Unfocus.
+
+SCase "sBranch_uncond".
+Focus.
+  destruct_ctx_other.
+  apply cmds_simulation_nil_inv in Hcssim2; subst.
+  inv Hop2.
+  uniq_result.
+
+  assert (block_simulation pinfo sasinfo F (block_intro l' ps' cs' tmn')
+           (block_intro l'0 ps'0 cs'0 tmn'0)) as Hbsim.
+    eauto using fdef_sim__block_sim.         
+  assert (uniqFdef F) as Huniq. eauto using wf_system__uniqFdef.
+  assert (blockInFdefB (block_intro l' ps' cs' tmn') F) as HBinF1'.
+    admit.  
+  assert (Hbsim':=Hbsim).
+  apply block_simulation_inv in Hbsim'; auto.
+  destruct Hbsim' as [Heq1 [Heq2 [Hcssim' Heq5]]]; subst.
+
+  assert (lc' = lc'0) as Heq.
+    clear - H0 H17 Hbsim2.
+    eapply switchToNewBasicBlock_sim in Hbsim2; eauto.
+  subst.
+
+  repeat_solve.
+    exists l'0. exists ps'0. exists nil. auto.
+    exists l'0. exists ps'0. exists nil. auto.
+  
+    clear - H0 Hmsim.
+    eapply switchToNewBasicBlock_Mem_simulation; eauto.
+
+Unfocus.
+
 Admitted.
+(*
+
+SCase "sBop". 
+(*
+Lemma mem_simulation_update_locals : 
+  forall pinfo sasinfo TD EC1 EC2 ECs M1 M2
+  (EQ: Opsem.CurFunction EC1 = Opsem.CurFunction EC2)
+  (Hp: forall gvsa
+   (Hlkup: lookupAL (GVsT DGVs) (Opsem.Locals EC1) (PI_id pinfo) = ret gvsa),
+   lookupAL (GVsT DGVs) (Opsem.Locals EC2) (PI_id pinfo) = ret gvsa)
+  (Hmsim: Mem_simulation pinfo sasinfo TD (EC1 :: ECs) M1 M2),
+  Mem_simulation pinfo sasinfo TD (EC2 :: ECs) M1 M2.
+Proof.
+  intros.
+  destruct Hmsim as [Hmsim1 Hmsim2].
+  split; auto.
+    intros.
+    eapply Hmsim2 with (ptr:=ptr)(ty:=ty)(al:=al); eauto.
+Admitted.    
+*)
+abstract (destruct_ctx_other; dse_is_sim_common_case).
+SCase "sFBop". abstract (destruct_ctx_other; dse_is_sim_common_case).
+SCase "sExtractValue". abstract (destruct_ctx_other; dse_is_sim_common_case).
+SCase "sInsertValue". abstract (destruct_ctx_other; dse_is_sim_common_case).
+SCase "sMalloc". 
+ 
+  destruct_ctx_other.
+ 
+  apply cmds_simulation_nelim_cons_inv in Hcssim2; simpl; auto;
+  destruct Hcssim2 as [cs3' [Heq Hcssim2]]; subst;
+  inv Hop2; uniq_result.
+
+  assert (mb0 = mb) as EQ.
+    destruct Hmsim as [Hmsim _].
+    apply MemProps.malloc_result in H25.
+    apply MemProps.malloc_result in H2. subst. auto.
+  subst.
+  repeat_solve.
+
+    destruct Hmsim as [Hmsim1 Hmsim2].
+    split; auto.
+      apply MemProps.nextblock_malloc in H2.
+      apply MemProps.nextblock_malloc in H25.
+      rewrite <- H2. rewrite <- H25. rewrite Hmsim1. auto.
+
+      intros.
+      eapply Hmsim2 with (ptr:=ptr)(ty:=ty)(al:=al); eauto.
+      eapply no_alias_head_tail_update in Hnalias; eauto; simpl; auto.
+        intros. admit. (* id <> palloca *)
+
+        (* two cases, if ptr is mb or not, 
+           malloc_preserves_mload_inv needs to be extended. *)
+        admit. admit.
+
+SCase "sFree". 
+
+  destruct_ctx_other.
+ 
+  apply cmds_simulation_nelim_cons_inv in Hcssim2; auto.
+  destruct Hcssim2 as [cs3' [Heq Hcssim2]]; subst;
+  inv Hop2; uniq_result.
+
+  repeat_solve.
+    destruct Hmsim as [Hmsim1 Hmsim2].
+    split; auto.
+      apply MemProps.nextblock_free in H1.
+      apply MemProps.nextblock_free in H22.
+      rewrite <- H1. rewrite <- H22. rewrite Hmsim1. auto.
+
+      intros.
+      eapply Hmsim2 with (ptr:=ptr)(ty:=ty)(al:=al); 
+        eauto using MemProps.free_preserves_mload_inv.
+      eapply no_alias_head_tail_irrel in Hnalias; eauto; simpl; auto.
+
+SCase "sAlloca". 
+
+  destruct_ctx_other.
+ 
+  apply cmds_simulation_nelim_cons_inv in Hcssim2; simpl; auto;
+  destruct Hcssim2 as [cs3' [Heq Hcssim2]]; subst;
+  inv Hop2; uniq_result.
+
+  assert (mb0 = mb) as EQ.
+    destruct Hmsim as [Hmsim _].
+    apply MemProps.malloc_result in H25.
+    apply MemProps.malloc_result in H2. subst. auto.
+  subst.
+  repeat_solve.
+
+    destruct Hmsim as [Hmsim1 Hmsim2].
+    split; auto.
+      apply MemProps.nextblock_malloc in H2.
+      apply MemProps.nextblock_malloc in H25.
+      rewrite <- H2. rewrite <- H25. rewrite Hmsim1. auto.
+
+      intros.
+      eapply Hmsim2 with (ptr:=ptr)(ty:=ty)(al:=al); eauto.
+      eapply no_alias_head_tail_update in Hnalias; eauto; simpl; auto.
+        intros.
+        admit. (* if id = palloca, then lc2 cannot contain pid *)
+
+        (* two cases, if ptr is mb or not, 
+           malloc_preserves_mload_inv needs to be extended. *)
+        admit. admit. 
+
+SCase "sLoad". 
+  destruct_ctx_other.
+
+  apply cmds_simulation_nelim_cons_inv in Hcssim2; simpl; auto;
+  destruct Hcssim2 as [cs3' [Heq Hcssim2]]; subst;
+  inv Hop2; uniq_result.
+
+  assert (gv = gv0) as EQ.
+    admit. (* no load from pid *)
+  subst.
+  repeat_solve.
+
+    eapply mem_simulation_update_locals in Hmsim; simpl; eauto.
+      simpl. intros.
+      admit. (* lid <> pid *)
+
+SCase "sStore". 
+
+  destruct_ctx_other.
+ 
+  assert (PI_f pinfo = F -> 
+          store_in_cmd (PI_id pinfo) (insn_store sid t v1 v2 align0) = false)
+         as J.
+    clear - Hnrem. simpl in Hnrem.
+    destruct v2; auto.
+    intros. subst.
+    destruct (fdef_dec (PI_f pinfo) (PI_f pinfo)); try congruence.
+    simpl.
+    destruct (id_dec i0 (PI_id pinfo)); subst; auto.
+    destruct (id_dec (PI_id pinfo) (PI_id pinfo)); try congruence.
+    contradict Hnrem; auto.
+  apply cmds_simulation_nelim_cons_inv in Hcssim2; auto.
+  destruct Hcssim2 as [cs3' [Heq Hcssim2]]; subst;
+  inv Hop2; uniq_result.
+
+  repeat_solve.
+    destruct Hmsim as [Hmsim1 Hmsim2].
+    split; auto.
+      apply MemProps.nextblock_mstore in H3.
+      apply MemProps.nextblock_mstore in H28.
+      rewrite <- H3. rewrite <- H28. rewrite Hmsim1. auto.
+
+      intros.
+      eapply Hmsim2 with (ptr:=ptr)(ty:=ty)(al:=al); eauto.
+      eapply no_alias_head_tail_irrel in Hnalias; eauto; simpl; auto.
+        (* two cases, if ptr overlaps with stored ptr or not *)
+        admit. admit.
+
+SCase "sGEP". abstract (destruct_ctx_other; dse_is_sim_common_case).
+SCase "sTrunc". abstract (destruct_ctx_other; dse_is_sim_common_case).
+SCase "sExt". abstract (destruct_ctx_other; dse_is_sim_common_case).
+SCase "sCast". abstract (destruct_ctx_other; dse_is_sim_common_case).
+SCase "sIcmp". abstract (destruct_ctx_other; dse_is_sim_common_case).
+SCase "sFcmp". abstract (destruct_ctx_other; dse_is_sim_common_case).
+SCase "sSelect". 
+  destruct_ctx_other.
+
+  apply cmds_simulation_nelim_cons_inv in Hcssim2; simpl; auto;
+  destruct Hcssim2 as [cs3' [Heq Hcssim2]]; subst;
+  inv Hop2; uniq_result.
+
+  repeat_solve.
+    destruct (isGVZero (los,nts) c).
+      eapply mem_simulation_update_locals in Hmsim; simpl; eauto.
+        simpl. intros.
+        admit. (* lid <> pid *)
+      eapply mem_simulation_update_locals in Hmsim; simpl; eauto.
+        simpl. intros.
+        admit. (* lid <> pid *)
+
+SCase "sCall".
+
+  destruct_ctx_other.
+  assert (Hcssim2':=Hcssim2).
+  apply cmds_simulation_nelim_cons_inv in Hcssim2; auto.
+  destruct Hcssim2 as [cs3' [Heq Hcssim2]]; subst.
+
+  inv Hop2.
+
+  SSCase "SCall".
+
+  uniq_result.
+  assert (Hfsim1:=Hpsim).
+  eapply lookupFdefViaPtr__simulation in Hfsim1; eauto.
+
+  assert (Hbsim1:=Hfsim1).
+  eapply fdef_simulation__entry_block_simulation in Hbsim1; eauto.
+  assert (Hbsim1':=Hbsim1).
+  apply block_simulation_inv in Hbsim1'.
+  destruct Hbsim1' as [Heq' [Hpsim1' [Hcsim1' Htsim1']]]; subst.
+  repeat_solve.
+    exists l'0. exists ps'0. exists nil. auto.
+    exists l'0. exists ps'0. exists nil. auto.
+
+    apply fdef_simulation_inv in Hfsim1.
+    destruct Hfsim1 as [Heq _]. inv Heq. uniq_result.
+    auto.
+
+    destruct Hmsim as [Hmsim1 Hmsim2].
+    split; auto.
+      intros.
+      eapply Hmsim2 with (ptr:=ptr)(ty:=ty)(al:=al); eauto.
+      clear Hmsim2.
+      apply no_alias_head_tail_cons_and in Hnalias.
+      destruct Hnalias as [Hnalias1 Hnalias2]; auto.
+
+  SSCase "sExCall".
+
+  uniq_result.
+
+  clear - H28 H1 Hpsim.
+  eapply lookupFdefViaPtr__simulation_l2r in H1; eauto.
+  destruct H1 as [f2 [H1 H2]].
+  apply OpsemAux.lookupExFdecViaPtr_inversion in H28.
+  apply OpsemAux.lookupFdefViaPtr_inversion in H1.
+  destruct H28 as [fn [J1 [J2 J3]]].
+  destruct H1 as [fn' [J4 J5]].
+  uniq_result.   
+
+SCase "sExCall". 
+
+  destruct_ctx_other.
+  assert (Hcssim2':=Hcssim2).
+  apply cmds_simulation_nelim_cons_inv in Hcssim2; auto.
+  destruct Hcssim2 as [cs3' [Heq Hcssim2]]; subst.
+
+  inv Hop2.
+
+  SSCase "SCall".
+
+  uniq_result.
+
+  clear - H29 H1 Hpsim.
+  eapply lookupExFdecViaPtr__simulation_l2r in H1; eauto.
+  apply OpsemAux.lookupExFdecViaPtr_inversion in H1.
+  apply OpsemAux.lookupFdefViaPtr_inversion in H29.
+  destruct H1 as [fn [J1 [J2 J3]]].
+  destruct H29 as [fn' [J4 J5]].
+  uniq_result.   
+
+  SSCase "sExCall".
+
+  uniq_result.
+
+  assert (Hlkdec:=Hpsim).
+  eapply lookupExFdecViaPtr__simulation_l2r in Hlkdec; eauto.
+  uniq_result.
+  eapply callExternalFunction__Mem_simulation in Hmsim; eauto.
+  destruct Hmsim as [EQ Hmsim]; subst.
+  uniq_result.
+  repeat_solve.
+    eapply mem_simulation_update_locals in Hmsim; simpl; eauto.
+      simpl. intros. admit. (* cid <> pid *)
+    
+Transparent inscope_of_tmn inscope_of_cmd.
+
+Qed.
+*)
 
 Lemma s_genInitState__sas_State_simulation: forall pinfo sasinfo S1 S2 main 
   VarArgs cfg2 IS2,
